\documentclass[11pt]{article}

\begin{document}
\section*{Ex.1}
$$(((P \vee Q) \Rightarrow R) \wedge (R \vee (P \wedge \neg Q))) \wedge \neg R$$
Translate the implication to an or-clause:
$$((\neg(P \vee Q) \vee R) \wedge (R \vee (P \wedge \neg Q))) \neg R$$
De Morgan:
$$(((\neg P \wedge \neg Q) \vee R) \wedge (R \vee (P \wedge \neg Q))) \wedge \neg R$$
Remove contradicting statements ($(\neg P \wedge \neg Q)$ and $(P \wedge \neg Q)$ can never be true at the same time)):
$$(R \wedge R) \wedge \neg R$$
A literal AND the same literal is the same as just writing the literal:
$$R \wedge \neg R$$
We are ending up with a contradiction.
\end{document}